# imports: https://spec.edmcouncil.org/cdmc/ontology/Core

@prefix cdmc-cls: <https://spec.edmcouncil.org/cdmc/ontology/Classification/> .
@prefix dc: <http://purl.org/dc/elements/1.1/> .
@prefix owl: <http://www.w3.org/2002/07/owl#> .
@prefix rdf: <http://www.w3.org/1999/02/22-rdf-syntax-ns#> .
@prefix rdfs: <http://www.w3.org/2000/01/rdf-schema#> .
@prefix xsd: <http://www.w3.org/2001/XMLSchema#> .

<https://spec.edmcouncil.org/cdmc/ontology/Classification>
	a owl:Ontology ;
	owl:imports <https://spec.edmcouncil.org/cdmc/ontology/Core> ;
	owl:versionInfo "Created with TopBraid Composer" ;
	.

cdmc-cls:Authority
	a owl:Class ;
	rdfs:subClassOf cdmc-cls:DataClassification ;
	rdfs:label "Authority" ;
	rdfs:comment "A classification of the information within a data asset that indicates whether it is considered authoritative within the organization." ;
	rdfs:isDefinedBy <https://spec.edmcouncil.org/cdmc/ontology/Classification> ;
	.

cdmc-cls:ClassificationOccurrence
	a owl:Class ;
	rdfs:subClassOf owl:Thing ;
	rdfs:label "Classification Occurrence" ;
	rdfs:comment "An instance of applying a Data Classification to a Resource." ;
	dc:source "CDMC" ;
	rdfs:isDefinedBy <https://spec.edmcouncil.org/cdmc/ontology/Classification> ;
	.

cdmc-cls:DataClassification
	a owl:Class ;
	rdfs:subClassOf owl:Thing ;
	rdfs:label "Data Classification" ;
	rdfs:comment "A category that organizes data for its most effective and efficient use." ;
	dc:source
		"CDMC" ,
		"DCAM"
		;
	rdfs:isDefinedBy <https://spec.edmcouncil.org/cdmc/ontology/Classification> ;
	.

cdmc-cls:InformationCriticality
	a owl:Class ;
	rdfs:subClassOf cdmc-cls:DataClassification ;
	rdfs:label "Information Criticality" ;
	rdfs:comment "A classification of the degree to which an organization depends on a resource for the success of one or more business functions." ;
	rdfs:isDefinedBy <https://spec.edmcouncil.org/cdmc/ontology/Classification> ;
	.

cdmc-cls:InformationSensitivity
	a owl:Class ;
	rdfs:subClassOf cdmc-cls:DataClassification ;
	rdfs:label "Information Sensitivity" ;
	rdfs:comment "A classification of the information within a data asset that indicates the level of control and protection that must be applied to the asset due to the nature of the data and its sensitivity or importance to the organization or to the subject of the data" ;
	dc:source "CDMC" ;
	rdfs:isDefinedBy <https://spec.edmcouncil.org/cdmc/ontology/Classification> ;
	.

cdmc-cls:appliedClassification
	a owl:ObjectProperty ;
	rdfs:label "applied classification" ;
	rdfs:comment "The Data Classification that has been applied to a Resource." ;
	dc:source "CDMC" ;
	rdfs:domain cdmc-cls:ClassificationOccurrence ;
	rdfs:isDefinedBy <https://spec.edmcouncil.org/cdmc/ontology/Classification> ;
	rdfs:range cdmc-cls:DataClassification ;
	.

cdmc-cls:classifiedResource
	a owl:ObjectProperty ;
	rdfs:label "classified resource" ;
	rdfs:comment "The Resource to which a Data Classification has been applied." ;
	dc:source "CDMC" ;
	rdfs:domain cdmc-cls:ClassificationOccurrence ;
	rdfs:isDefinedBy <https://spec.edmcouncil.org/cdmc/ontology/Classification> ;
	rdfs:range <https://spec.edmcouncil.org/cdmc/ontology/Core/Resource> ;
	.

