# imports: https://spec.edmcouncil.org/cdmc/ontology/Core
# imports: https://spec.edmcouncil.org/cdmc/ontology/Lineage

@prefix cdmc-core: <https://spec.edmcouncil.org/cdmc/ontology/Core/> .
@prefix cdmc-cv: <https://spec.edmcouncil.org/cdmc/ontology/ControlledVocabularies/> .
@prefix dc: <http://purl.org/dc/elements/1.1/> .
@prefix owl: <http://www.w3.org/2002/07/owl#> .
@prefix rdf: <http://www.w3.org/1999/02/22-rdf-syntax-ns#> .
@prefix rdfs: <http://www.w3.org/2000/01/rdf-schema#> .
@prefix sm: <http://www.omg.org/techprocess/ab/SpecificationMetadata/> .
@prefix xsd: <http://www.w3.org/2001/XMLSchema#> .

<https://spec.edmcouncil.org/cdmc/ontology/ControlledVocabularies>
	a owl:Ontology ;
	owl:imports
		<https://spec.edmcouncil.org/cdmc/ontology/Core> ,
		<https://spec.edmcouncil.org/cdmc/ontology/Lineage>
		;
	owl:versionInfo "Created with TopBraid Composer" ;
	.

cdmc-cv:BusinessElement
	a owl:Class ;
	rdfs:subClassOf cdmc-cv:DataElementConcept ;
	rdfs:label "Business Element" ;
	rdfs:comment "A unit of information that has a specific meaning in the context of a business process or collection of processes within a data domain." ;
	dc:source "DCAM" ;
	rdfs:isDefinedBy <https://spec.edmcouncil.org/cdmc/ontology/ControlledVocabularies> ;
	.

cdmc-cv:BusinessGlossary
	a owl:Class ;
	rdfs:subClassOf cdmc-cv:ConceptGroup ;
	rdfs:label "Business Glossary" ;
	rdfs:comment "A collection of term names and definitions from the perspective of the business process." ;
	dc:source "DCAM" ;
	rdfs:isDefinedBy <https://spec.edmcouncil.org/cdmc/ontology/ControlledVocabularies> ;
	.

cdmc-cv:BusinessProcess
	a owl:Class ;
	rdfs:subClassOf <https://spec.edmcouncil.org/cdmc/ontology/Lineage/Activity> ;
	rdfs:label "Business Process" ;
	rdfs:comment "An activity or set of activities that can accomplish a specific organizational goal." ;
	dc:source "CDMC" ;
	rdfs:isDefinedBy <https://spec.edmcouncil.org/cdmc/ontology/ControlledVocabularies> ;
	cdmc-core:field_reference <https://searchcio.techtarget.com/definition/business-process> ;
	.

cdmc-cv:Class
	a owl:Class ;
	rdfs:subClassOf owl:Thing ;
	rdfs:label "Class" ;
	rdfs:comment "A description of a set of objects that share the same attributes, operations, methods, relationships, and semantics." ;
	dc:source <https://iso.org/iso-11179/v0/> ;
	rdfs:isDefinedBy <https://spec.edmcouncil.org/cdmc/ontology/ControlledVocabularies> ;
	rdfs:seeAlso <https://iso.org/iso-11179/v0/Class> ;
	.

cdmc-cv:Concept
	a owl:Class ;
	rdfs:subClassOf cdmc-core:Resource ;
	rdfs:label "Concept" ;
	rdfs:comment "A unit of knowledge created by a unique combination of characteristics." ;
	dc:source <https://iso.org/iso-11179/v0/> ;
	rdfs:isDefinedBy <https://spec.edmcouncil.org/cdmc/ontology/ControlledVocabularies> ;
	rdfs:seeAlso
		<http://www.w3.org/2004/02/skos/core#Concept> ,
		<https://iso.org/iso-11179/v0/Concept> ,
		<https://iso.org/iso-25964/v0/Concept>
		;
	.

cdmc-cv:ConceptGroup
	a owl:Class ;
	rdfs:subClassOf owl:Thing ;
	rdfs:label "Concept Group" ;
	rdfs:comment "An aggregation of one or more concepts. Semantic relationships (links) between those concepts may also be viewed as part of a concept scheme. This definition is, however, meant to be suggestive rather than restrictive, and there is some flexibility in the formal data model stated below." ;
	rdfs:isDefinedBy <https://spec.edmcouncil.org/cdmc/ontology/ControlledVocabularies> ;
	rdfs:seeAlso
		<http://www.w3.org/2004/02/skos/core#ConceptScheme> ,
		<https://iso.org/iso-25964/v0/ConceptGroup>
		;
	.

cdmc-cv:ConceptualDomain
	a owl:Class ;
	rdfs:subClassOf owl:Thing ;
	rdfs:label "Conceptual Domain" ;
	rdfs:comment "A set of concepts, not necessarily finite, where the concepts represent the meaning of the permissible values in a value domain." ;
	dc:source <https://iso.org/iso-11179/v0/> ;
	rdfs:isDefinedBy <https://spec.edmcouncil.org/cdmc/ontology/ControlledVocabularies> ;
	rdfs:seeAlso <https://iso.org/iso-11179/v0/ConceptualDomain> ;
	cdmc-core:field_reference <https://www.iso.org/obp/ui/#iso:std:iso-iec:11179:-1:ed-3:v1:en> ;
	.

cdmc-cv:DataAttribute
	a owl:Class ;
	rdfs:subClassOf owl:Thing ;
	rdfs:label "Data Attribute" ;
	rdfs:isDefinedBy <https://spec.edmcouncil.org/cdmc/ontology/ControlledVocabularies> ;
	.

cdmc-cv:DataElement
	a owl:Class ;
	rdfs:subClassOf
		cdmc-core:Resource ,
		_:blank6 ,
		_:blank7
		;
	rdfs:label "Data Element" ;
	rdfs:comment "A unit of data that is considered in context to be indivisible." ;
	dc:source <https://iso.org/iso-11179/v0/> ;
	rdfs:isDefinedBy <https://spec.edmcouncil.org/cdmc/ontology/ControlledVocabularies> ;
	rdfs:seeAlso <https://iso.org/iso-11179/v0/DataElement> ;
	.

cdmc-cv:DataElementConcept
	a owl:Class ;
	rdfs:subClassOf cdmc-cv:Concept ;
	rdfs:label "Data Element Concept" ;
	rdfs:comment "A concept that can be represented in the form of a data element, described independently of any particular representation." ;
	dc:source <https://iso.org/iso-11179/v0/> ;
	rdfs:isDefinedBy <https://spec.edmcouncil.org/cdmc/ontology/ControlledVocabularies> ;
	rdfs:seeAlso
		<https://iso.org/iso-11179/v0/DataElementConcept> ,
		<https://iso.org/iso-25964/v0/DataElementConcept>
		;
	.

cdmc-cv:DataEntity
	a owl:Class ;
	rdfs:subClassOf
		cdmc-cv:Concept ,
		_:blank8
		;
	rdfs:label "Data Entity" ;
	rdfs:comment "A concept that represents a person, place or thing." ;
	dc:source "DCAM" ;
	rdfs:isDefinedBy <https://spec.edmcouncil.org/cdmc/ontology/ControlledVocabularies> ;
	.

cdmc-cv:DataModel
	a owl:Class ;
	rdfs:subClassOf
		cdmc-core:Resource ,
		_:blank3
		;
	rdfs:label "Data Model" ;
	rdfs:comment "A model that presents the declarative structure of data through a defined scope and perspective, and to a given level of abstraction." ;
	dc:source "DCAM" ;
	rdfs:isDefinedBy <https://spec.edmcouncil.org/cdmc/ontology/ControlledVocabularies> ;
	.

cdmc-cv:OperationalProcess
	a owl:Class ;
	rdfs:subClassOf
		owl:Thing ,
		_:blank2
		;
	rdfs:label "Operational Process" ;
	rdfs:comment "An activity or set of activities that can accomplish a specific operational outcome." ;
	dc:source "CDMC" ;
	rdfs:isDefinedBy <https://spec.edmcouncil.org/cdmc/ontology/ControlledVocabularies> ;
	.

cdmc-cv:Property
	a owl:Class ;
	rdfs:subClassOf owl:Thing ;
	rdfs:label "Property" ;
	rdfs:comment "A characteristic common to all members of a Class." ;
	dc:source
		"CDMC" ,
		"iso-11179:"
		;
	rdfs:isDefinedBy <https://spec.edmcouncil.org/cdmc/ontology/ControlledVocabularies> ;
	<https://iso.org/iso-11179/v0/Property> "" ;
	.

cdmc-cv:SubjectArea
	a owl:Class ;
	rdfs:subClassOf owl:Thing ;
	rdfs:label "subject area" ;
	rdfs:isDefinedBy <https://spec.edmcouncil.org/cdmc/ontology/ControlledVocabularies> ;
	.

cdmc-cv:Thesaurus
	a owl:Class ;
	rdfs:subClassOf cdmc-cv:BusinessGlossary ;
	rdfs:label "Thesaurus" ;
	rdfs:comment "A Business Glossary that includes synonyms between terms." ;
	dc:source "CDMC" ;
	rdfs:isDefinedBy <https://spec.edmcouncil.org/cdmc/ontology/ControlledVocabularies> ;
	.

cdmc-cv:ValueDomain
	a owl:Class ;
	rdfs:subClassOf
		owl:Thing ,
		_:blank5
		;
	rdfs:label "Value Domain" ;
	rdfs:comment "Contains the allowed values for a data element." ;
	dc:source <https://iso.org/iso-11179/v0/> ;
	rdfs:isDefinedBy <https://spec.edmcouncil.org/cdmc/ontology/ControlledVocabularies> ;
	rdfs:seeAlso <https://iso.org/iso-11179/v0/ValueDomain> ;
	cdmc-core:field_reference <https://www.iso.org/obp/ui/#iso:std:iso-iec:11179:-1:ed-3:v1:en> ;
	.

cdmc-cv:Workflow
	a owl:Class ;
	rdfs:subClassOf
		owl:Thing ,
		_:blank4
		;
	rdfs:label "Workflow" ;
	rdfs:comment "A sequence of events through which a Business Process progresses from initiation to completion." ;
	dc:source
		"CDMC" ,
		<https://www.oed.com>
		;
	rdfs:isDefinedBy <https://spec.edmcouncil.org/cdmc/ontology/ControlledVocabularies> ;
	.

cdmc-cv:composedOf
	a owl:ObjectProperty ;
	rdfs:label "composed of" ;
	rdfs:comment "Business Processes can be hierarchical in nature, and this relationship reflects the composition of complex Business Processes out of simpler ones." ;
	dc:source "CDMC" ;
	rdfs:domain cdmc-cv:BusinessProcess ;
	rdfs:isDefinedBy <https://spec.edmcouncil.org/cdmc/ontology/ControlledVocabularies> ;
	rdfs:range cdmc-cv:BusinessProcess ;
	.

cdmc-cv:forClass
	a owl:ObjectProperty ;
	rdfs:label "for class" ;
	rdfs:comment "The Class for which this Data Element Concept binds a particular Property." ;
	dc:source "CDMC" ;
	rdfs:domain cdmc-cv:DataElementConcept ;
	rdfs:isDefinedBy <https://spec.edmcouncil.org/cdmc/ontology/ControlledVocabularies> ;
	rdfs:range cdmc-cv:Class ;
	.

cdmc-cv:forProperty
	a owl:ObjectProperty ;
	rdfs:label "for property" ;
	rdfs:comment "The Property that is bound to a Class by this Data Element Concept." ;
	dc:source "CDMC" ;
	rdfs:domain cdmc-cv:DataElementConcept ;
	rdfs:isDefinedBy <https://spec.edmcouncil.org/cdmc/ontology/ControlledVocabularies> ;
	rdfs:range cdmc-cv:Property ;
	.

cdmc-cv:hasAttribute
	a owl:ObjectProperty ;
	rdfs:label "has attribute" ;
	rdfs:domain cdmc-cv:DataEntity ;
	rdfs:isDefinedBy <https://spec.edmcouncil.org/cdmc/ontology/ControlledVocabularies> ;
	rdfs:range cdmc-cv:DataAttribute ;
	.

cdmc-cv:hasBroaderConcept
	a owl:ObjectProperty ;
	rdfs:label "has broader concept" ;
	rdfs:comment "A concept that is more general in meaning than this one." ;
	dc:source <http://www.w3.org/2004/02/skos/core#> ;
	rdfs:domain cdmc-cv:Concept ;
	rdfs:isDefinedBy <https://spec.edmcouncil.org/cdmc/ontology/ControlledVocabularies> ;
	rdfs:range cdmc-cv:Concept ;
	rdfs:seeAlso <http://www.w3.org/2004/02/skos/core#broader> ;
	.

cdmc-cv:hasConceptualDomain
	a owl:ObjectProperty ;
	rdfs:label "has conceptual domain" ;
	rdfs:comment "The Conceptual Domain that covers this Data Element Concept." ;
	dc:source "CDMC" ;
	rdfs:domain cdmc-cv:DataElementConcept ;
	rdfs:isDefinedBy <https://spec.edmcouncil.org/cdmc/ontology/ControlledVocabularies> ;
	rdfs:range cdmc-cv:ConceptualDomain ;
	.

cdmc-cv:hasInput
	a owl:ObjectProperty ;
	rdfs:label "has input" ;
	rdfs:comment "A Data Element that is an input to this Workflow." ;
	dc:source "CDMC" ;
	rdfs:domain cdmc-cv:Workflow ;
	rdfs:isDefinedBy <https://spec.edmcouncil.org/cdmc/ontology/ControlledVocabularies> ;
	rdfs:range cdmc-cv:DataElement ;
	.

cdmc-cv:hasSubject
	a owl:ObjectProperty ;
	rdfs:label "has subject" ;
	rdfs:domain cdmc-cv:DataModel ;
	rdfs:isDefinedBy <https://spec.edmcouncil.org/cdmc/ontology/ControlledVocabularies> ;
	rdfs:range cdmc-cv:SubjectArea ;
	.

cdmc-cv:hasTheme
	a owl:ObjectProperty ;
	rdfs:label "has theme" ;
	rdfs:comment "A main category of the entity." ;
	dc:source
		"CDMC" ,
		<http://www.w3.org/ns/dcat#>
		;
	rdfs:domain <https://spec.edmcouncil.org/cdmc/ontology/Lineage/Entity> ;
	rdfs:isDefinedBy <https://spec.edmcouncil.org/cdmc/ontology/Lineage> ;
	rdfs:range cdmc-cv:Concept ;
	rdfs:seeAlso <http://www.w3.org/ns/dcat#theme> ;
	.

cdmc-cv:hasThemes
	a owl:ObjectProperty ;
	rdfs:label "has themes" ;
	rdfs:comment "A collection of concepts that describe, topically, the contents of a catalog." ;
	rdfs:domain cdmc-core:Catalog ;
	rdfs:isDefinedBy <https://spec.edmcouncil.org/cdmc/ontology/Core> ;
	rdfs:range cdmc-cv:ConceptGroup ;
	.

cdmc-cv:hasTopConcept
	a owl:ObjectProperty ;
	rdfs:label "has top concept" ;
	rdfs:comment "The property skos:hasTopConcept is, by convention, used to link a concept scheme to the SKOS concept(s) which are topmost in the hierarchical relations for that scheme." ;
	dc:source <http://www.w3.org/2004/02/skos/core#> ;
	rdfs:domain cdmc-cv:ConceptGroup ;
	rdfs:isDefinedBy <https://spec.edmcouncil.org/cdmc/ontology/ControlledVocabularies> ;
	rdfs:range cdmc-cv:Concept ;
	.

cdmc-cv:hasValueDomain
	a owl:ObjectProperty ;
	rdfs:label "has value domain" ;
	rdfs:comment "The Value Domain of valid values for this Data Element." ;
	dc:source "CDMC" ;
	rdfs:domain cdmc-cv:DataElement ;
	rdfs:isDefinedBy <https://spec.edmcouncil.org/cdmc/ontology/ControlledVocabularies> ;
	rdfs:range cdmc-cv:ValueDomain ;
	.

cdmc-cv:inConceptGroup
	a owl:ObjectProperty ;
	rdfs:label "in concept group" ;
	rdfs:comment "A concept group in which this concept is included." ;
	dc:source
		"CDMC" ,
		<http://www.w3.org/2004/02/skos/core#>
		;
	rdfs:domain cdmc-cv:Concept ;
	rdfs:isDefinedBy <https://spec.edmcouncil.org/cdmc/ontology/ControlledVocabularies> ;
	rdfs:range cdmc-cv:ConceptGroup ;
	rdfs:seeAlso <http://www.w3.org/2004/02/skos/core#inScheme> ;
	.

cdmc-cv:isRelatedTo
	a owl:ObjectProperty ;
	rdfs:label "is related to" ;
	rdfs:comment "Signifies a semantic relationship between Concepts." ;
	dc:source "CDMC" ;
	rdfs:domain cdmc-cv:Concept ;
	rdfs:isDefinedBy <https://spec.edmcouncil.org/cdmc/ontology/ControlledVocabularies> ;
	rdfs:range cdmc-cv:Concept ;
	.

cdmc-cv:modeledAs
	a owl:ObjectProperty ;
	rdfs:label "modeled as" ;
	rdfs:comment "The modelling of a Data Element Concept as a Data Attribute" ;
	rdfs:domain cdmc-cv:DataElementConcept ;
	rdfs:isDefinedBy <https://spec.edmcouncil.org/cdmc/ontology/ControlledVocabularies> ;
	rdfs:range cdmc-cv:DataAttribute ;
	.

cdmc-cv:usesDataElementConcept
	a owl:ObjectProperty ;
	rdfs:label "uses data element concept" ;
	rdfs:comment "A Data Element Concept used by this Business Process." ;
	dc:source "CDMC" ;
	rdfs:domain cdmc-cv:BusinessProcess ;
	rdfs:isDefinedBy <https://spec.edmcouncil.org/cdmc/ontology/ControlledVocabularies> ;
	rdfs:range cdmc-cv:DataElementConcept ;
	.

cdmc-core:DataSet
	rdfs:subClassOf _:blank1 ;
	.

_:blank1
	a owl:Restriction ;
	owl:onProperty cdmc-core:contains ;
	owl:someValuesFrom cdmc-cv:DataElement ;
	.

_:blank2
	a owl:Restriction ;
	owl:onProperty cdmc-core:contains ;
	owl:someValuesFrom <https://spec.edmcouncil.org/cdmc/ontology/Lineage/Activity> ;
	.

_:blank3
	a owl:Restriction ;
	owl:onProperty cdmc-core:describes ;
	owl:someValuesFrom cdmc-core:DataAsset ;
	.

_:blank4
	a owl:Restriction ;
	owl:onProperty cdmc-core:implements ;
	owl:someValuesFrom cdmc-cv:BusinessProcess ;
	.

_:blank5
	a owl:Restriction ;
	owl:onProperty cdmc-core:implements ;
	owl:someValuesFrom cdmc-cv:ConceptualDomain ;
	.

_:blank6
	a owl:Restriction ;
	owl:onProperty cdmc-core:implements ;
	owl:someValuesFrom cdmc-cv:DataAttribute ;
	.

_:blank7
	a owl:Restriction ;
	owl:onProperty cdmc-core:implements ;
	owl:someValuesFrom cdmc-cv:DataElementConcept ;
	.

_:blank8
	a owl:Restriction ;
	owl:onProperty cdmc-core:isPartOf ;
	owl:someValuesFrom cdmc-cv:DataModel ;
	.

