# imports: https://spec.edmcouncil.org/cdmc/ontology/Classification
# imports: https://spec.edmcouncil.org/cdmc/ontology/Core

@prefix cdmc-cls: <https://spec.edmcouncil.org/cdmc/ontology/Classification/> .
@prefix cdmc-core: <https://spec.edmcouncil.org/cdmc/ontology/Core/> .
@prefix cdmc-ctl: <https://spec.edmcouncil.org/cdmc/ontology/Control/> .
@prefix dct: <http://purl.org/dc/terms/> .
@prefix owl: <http://www.w3.org/2002/07/owl#> .
@prefix rdf: <http://www.w3.org/1999/02/22-rdf-syntax-ns#> .
@prefix rdfs: <http://www.w3.org/2000/01/rdf-schema#> .
@prefix skos: <http://www.w3.org/2004/02/skos/core#> .
@prefix sm: <http://www.omg.org/techprocess/ab/SpecificationMetadata/> .
@prefix xsd: <http://www.w3.org/2001/XMLSchema#> .

<https://spec.edmcouncil.org/cdmc/ontology/Control>
	a owl:Ontology ;
	dct:abstract "This ontology defines terms and constructis for measurement and control of data in the cloud. " ;
	dct:license "https://opensource.org/licenses/MIT"^^xsd:AnyURI ;
	sm:copyright "Copyright (c) 2022 EDM Council, Inc." ;
	owl:imports
		<https://spec.edmcouncil.org/cdmc/ontology/Classification> ,
		<https://spec.edmcouncil.org/cdmc/ontology/Core>
		;
	owl:versionInfo "Created with TopBraid Composer" ;
	.

cdmc-ctl:Control
	a owl:Class ;
	rdfs:subClassOf owl:Thing ;
	rdfs:label "Control" ;
	rdfs:isDefinedBy <https://spec.edmcouncil.org/cdmc/ontology/Control> ;
	skos:definition "defined way to ensure control of Data Assets" ;
	.

cdmc-ctl:ControlInstance
	a owl:Class ;
	rdfs:subClassOf
		owl:Thing ,
		_:blank4 ,
		_:blank5
		;
	rdfs:label "Control Instance" ;
	rdfs:isDefinedBy <https://spec.edmcouncil.org/cdmc/ontology/Control> ;
	skos:definition "implementation of a Control for a Data Asset" ;
	.

cdmc-ctl:ControlMetric
	a owl:Class ;
	rdfs:subClassOf cdmc-core:Metric ;
	rdfs:label "Control Metric" ;
	rdfs:isDefinedBy <https://spec.edmcouncil.org/cdmc/ontology/Control> ;
	skos:definition "definition of a measurement that determines the effectiveness of a Control" ;
	.

cdmc-ctl:ControlMetricMeasurement
	a owl:Class ;
	rdfs:subClassOf owl:Thing ;
	rdfs:label "Control Metric Measurement" ;
	rdfs:isDefinedBy <https://spec.edmcouncil.org/cdmc/ontology/Control> ;
	skos:definition "value of a Control Metric at a point in time" ;
	.

cdmc-ctl:ControlMetricThreshold
	a owl:Class ;
	rdfs:subClassOf owl:Thing ;
	rdfs:label "Control Metric Threshold" ;
	rdfs:isDefinedBy <https://spec.edmcouncil.org/cdmc/ontology/Control> ;
	skos:definition "value against which a Control Metric Measurement is compared to assess the effectiveness of a Control" ;
	.

cdmc-ctl:SecurityControl
	a owl:Class ;
	rdfs:subClassOf
		cdmc-ctl:Control ,
		_:blank1
		;
	rdfs:label "Security Control" ;
	rdfs:isDefinedBy <https://spec.edmcouncil.org/cdmc/ontology/Control> ;
	skos:definition "safeguard or countermeasure meeting a set of defined security requirements to protect data" ;
	.

cdmc-ctl:SecurityControlInstance
	a owl:Class ;
	rdfs:subClassOf
		cdmc-ctl:ControlInstance ,
		_:blank2 ,
		_:blank3
		;
	rdfs:label "Security Control Instance" ;
	rdfs:isDefinedBy <https://spec.edmcouncil.org/cdmc/ontology/Control> ;
	skos:definition "implementation of a Security Control for a specific Data Service or Database Storage instance" ;
	.

cdmc-ctl:ThresholdConstraint
	a owl:Class ;
	rdfs:subClassOf owl:Thing ;
	rdfs:label "Threshold Constraint" ;
	rdfs:isDefinedBy <https://spec.edmcouncil.org/cdmc/ontology/Control> ;
	skos:definition "relationship between a Control Metric Measurement and the corresponding Control Metric Threshold that determines the effectiveness of a Control" ;
	.

cdmc-ctl:hasConstraintType
	a owl:ObjectProperty ;
	rdfs:label "has constraint type" ;
	rdfs:domain cdmc-ctl:ControlMetricThreshold ;
	rdfs:isDefinedBy <https://spec.edmcouncil.org/cdmc/ontology/Control> ;
	rdfs:range cdmc-ctl:ThresholdConstraint ;
	skos:definition "specifies the Threshold Constraint that applies to the Control Metric Threshold of a Control Metric" ;
	.

cdmc-ctl:hasLimitOf
	a owl:ObjectProperty ;
	rdfs:label "has limit of" ;
	rdfs:domain cdmc-ctl:ControlMetric ;
	rdfs:isDefinedBy <https://spec.edmcouncil.org/cdmc/ontology/Control> ;
	rdfs:range cdmc-ctl:ControlMetricThreshold ;
	skos:definition "indicates the use of a Control Metric Threshold as a limit against which the Control Metric Measurement of a Control can be compared" ;
	.

cdmc-ctl:isEvidencedBy
	a owl:ObjectProperty ;
	rdfs:label "is evidenced by" ;
	rdfs:domain cdmc-ctl:ControlInstance ;
	rdfs:isDefinedBy <https://spec.edmcouncil.org/cdmc/ontology/Control> ;
	rdfs:range cdmc-ctl:ControlMetricMeasurement ;
	skos:definition "indicates the use of a Control Metric Measurement to evidence of the existence of a Control Instance" ;
	.

cdmc-ctl:isMeasuredBy
	a owl:ObjectProperty ;
	rdfs:label "is measured by" ;
	rdfs:domain cdmc-ctl:Control ;
	rdfs:isDefinedBy <https://spec.edmcouncil.org/cdmc/ontology/Control> ;
	rdfs:range cdmc-ctl:ControlMetric ;
	skos:definition "indicates the use of a Control Metric to measure the effectiveness of a Control" ;
	.

cdmc-ctl:isMeasurementOf
	a owl:ObjectProperty ;
	rdfs:label "is measurement of" ;
	rdfs:domain cdmc-ctl:ControlMetricMeasurement ;
	rdfs:isDefinedBy <https://spec.edmcouncil.org/cdmc/ontology/Control> ;
	rdfs:range cdmc-ctl:ControlMetric ;
	skos:definition "identifies the Control Metric to which a Control Metric Measurement applies" ;
	.

_:blank1
	a owl:Restriction ;
	owl:onProperty cdmc-core:appliesTo ;
	owl:someValuesFrom cdmc-cls:InformationSensitivity ;
	.

_:blank2
	a owl:Restriction ;
	owl:onProperty cdmc-core:appliesTo ;
	owl:someValuesFrom cdmc-core:DataService ;
	.

_:blank3
	a owl:Restriction ;
	owl:onProperty cdmc-core:appliesTo ;
	owl:someValuesFrom cdmc-core:DatabaseStorage ;
	.

_:blank4
	a owl:Restriction ;
	owl:onProperty cdmc-core:appliesTo ;
	owl:someValuesFrom cdmc-core:Resource ;
	.

_:blank5
	a owl:Restriction ;
	owl:onProperty cdmc-core:implements ;
	owl:someValuesFrom cdmc-ctl:Control ;
	.

