# imports: http://purl.org/dc/elements/1.1/

@prefix cdmc-core: <https://spec.edmcouncil.org/cdmc/ontology/Core/> .
@prefix dc: <http://purl.org/dc/elements/1.1/> .
@prefix dct: <http://purl.org/dc/terms/> .
@prefix owl: <http://www.w3.org/2002/07/owl#> .
@prefix rdf: <http://www.w3.org/1999/02/22-rdf-syntax-ns#> .
@prefix rdfs: <http://www.w3.org/2000/01/rdf-schema#> .
@prefix sm: <http://www.omg.org/techprocess/ab/SpecificationMetadata/> .
@prefix xsd: <http://www.w3.org/2001/XMLSchema#> .

<https://spec.edmcouncil.org/cdmc/ontology/Core>
	a owl:Ontology ;
	dct:abstract "This ontology about the basic concepts that are important for cloud data management, and are used in the other CDMC ontologies. " ;
	dct:license "https://opensource.org/licenses/MIT"^^xsd:AnyURI ;
	sm:copyright "Copyright (c) 2022 EDM Council, Inc." ;
	owl:imports <http://purl.org/dc/elements/1.1/> ;
	owl:versionInfo "Created with TopBraid Composer" ;
	.

cdmc-core:Agent
	a owl:Class ;
	rdfs:label "Agent" ;
	rdfs:comment "something that bears some form of responsibility for an activity taking place" ;
	dc:source <http://www.w3.org/ns/prov#> ;
	rdfs:isDefinedBy <https://spec.edmcouncil.org/cdmc/ontology/Core> ;
	rdfs:seeAlso
		"egeria:ActorProfile" ,
		dc:Agent ,
		<http://www.w3.org/ns/odrl/2/Party> ,
		<http://www.w3.org/ns/prov#Agent> ,
		<http://xmlns.com/foaf/0.1/Agent>
		;
	.

cdmc-core:AgentInRole
	a owl:Class ;
	rdfs:subClassOf owl:Thing ;
	rdfs:label "Agent In Role" ;
	rdfs:comment "fulfilment of a specified role by an agent" ;
	rdfs:isDefinedBy <https://spec.edmcouncil.org/cdmc/ontology/Core> ;
	.

cdmc-core:Api
	a owl:Class ;
	rdfs:subClassOf cdmc-core:DataService ;
	rdfs:label "API" ;
	rdfs:comment "abstract set of methods that can be used to interface with a computer system" ;
	dc:source "CDMC" ;
	rdfs:isDefinedBy <https://spec.edmcouncil.org/cdmc/ontology/Core> ;
	.

cdmc-core:Catalog
	a owl:Class ;
	rdfs:subClassOf
		owl:Thing ,
		_:blank8
		;
	rdfs:label "Catalog" ;
	rdfs:comment "curated collection of metadata about resources (e.g., datasets and data services in the context of a data catalog)" ;
	dc:source <http://www.w3.org/ns/dcat#> ;
	rdfs:isDefinedBy <https://spec.edmcouncil.org/cdmc/ontology/Core> ;
	rdfs:seeAlso <http://www.w3.org/ns/dcat#Catalog> ;
	.

cdmc-core:CatalogRecord
	a owl:Class ;
	rdfs:subClassOf owl:Thing ;
	rdfs:label "Catalog Record" ;
	rdfs:comment "record in a catalog, describing the registration of a single dcat:Resource" ;
	dc:source <http://www.w3.org/ns/dcat#> ;
	rdfs:isDefinedBy <https://spec.edmcouncil.org/cdmc/ontology/Core> ;
	rdfs:seeAlso <http://www.w3.org/ns/dcat#CatalogRecord> ;
	.

cdmc-core:DataAsset
	a owl:Class ;
	rdfs:subClassOf cdmc-core:Resource ;
	rdfs:label "Data Asset" ;
	rdfs:comment "data asset is any collection of data owned by an organization that is considered to have intrinsic value" ;
	dc:source "DCAM Glossary" ;
	rdfs:isDefinedBy <https://spec.edmcouncil.org/cdmc/ontology/Core> ;
	rdfs:seeAlso
		"egeria:Asset" ,
		<http://www.w3.org/ns/odrl/2/Asset>
		;
	.

cdmc-core:DataService
	a owl:Class ;
	rdfs:subClassOf cdmc-core:Resource ;
	rdfs:label "Data Service" ;
	rdfs:comment "collection of operations that provides access to one or more datasets or data processing functions" ;
	dc:source <http://www.w3.org/ns/dcat#> ;
	rdfs:isDefinedBy <https://spec.edmcouncil.org/cdmc/ontology/Core> ;
	rdfs:seeAlso <http://www.w3.org/ns/dcat#DataService> ;
	.

cdmc-core:DataSet
	a owl:Class ;
	rdfs:subClassOf cdmc-core:DataAsset ;
	rdfs:label "Data Set" ;
	rdfs:comment "organized collection of data made available for consumption" ;
	dc:source "DCAM Glossary" ;
	rdfs:isDefinedBy <https://spec.edmcouncil.org/cdmc/ontology/Core> ;
	rdfs:seeAlso
		"egeria:DataSet" ,
		<http://www.w3.org/ns/dcat#Dataset>
		;
	.

cdmc-core:DatabaseAccessService
	a owl:Class ;
	rdfs:subClassOf cdmc-core:DataService ;
	rdfs:label "Database Access Service" ;
	rdfs:comment "organized collection of data stored and accessed electronically from a computer system" ;
	dc:source "CDMC" ;
	rdfs:isDefinedBy <https://spec.edmcouncil.org/cdmc/ontology/Core> ;
	cdmc-core:field_reference "PC.com" ;
	.

cdmc-core:DatabaseStorage
	a owl:Class ;
	rdfs:subClassOf owl:Thing ;
	rdfs:label "Database Storage" ;
	rdfs:comment "physical media on which the serialization of a data set is persisted" ;
	rdfs:isDefinedBy <https://spec.edmcouncil.org/cdmc/ontology/Core> ;
	.

cdmc-core:Distribution
	a owl:Class ;
	rdfs:subClassOf owl:Thing ;
	rdfs:label "Distribution" ;
	rdfs:comment "specific representation of a dataset. A dataset might be available in multiple serializations that may differ in various ways, including natural language, media-type or format, schematic organization, temporal and spatial resolution, level of detail or profiles (which might specify any or all of the above)" ;
	dc:source <http://www.w3.org/ns/dcat#> ;
	rdfs:isDefinedBy <https://spec.edmcouncil.org/cdmc/ontology/Core> ;
	rdfs:seeAlso <http://www.w3.org/ns/dcat#Distribution> ;
	.

cdmc-core:Location
	a owl:Class ;
	rdfs:subClassOf owl:Thing ;
	rdfs:label "Location" ;
	rdfs:comment "location can be an identifiable geographic place (ISO 19112), but it can also be a non-geographic place such as a directory, row, or column. As such, there are numerous ways in which location can be expressed, such as by a coordinate, address, landmark, and so forth" ;
	dc:source <http://www.w3.org/ns/prov#> ;
	rdfs:isDefinedBy <https://spec.edmcouncil.org/cdmc/ontology/Core> ;
	.

cdmc-core:MediaType
	a owl:Class ;
	rdfs:subClassOf owl:Thing ;
	rdfs:label "Media Type" ;
	rdfs:comment "indicator of the nature and format of a document, file, or assortment of bytes" ;
	dc:source <http://www.w3.org/ns/dcat#> ;
	rdfs:isDefinedBy <https://spec.edmcouncil.org/cdmc/ontology/Core> ;
	rdfs:seeAlso <https://www.iana.org/assignments/media-types> ;
	.

cdmc-core:Metric
	a owl:Class ;
	rdfs:subClassOf owl:Thing ;
	rdfs:label "Metric" ;
	rdfs:comment "measure of quantitative assessment" ;
	rdfs:isDefinedBy <https://spec.edmcouncil.org/cdmc/ontology/Core> ;
	.

cdmc-core:PeriodOfTime
	a owl:Class ;
	rdfs:subClassOf owl:Thing ;
	rdfs:label "Period of Time" ;
	rdfs:comment "interval of time that is named or defined by its start and end dates" ;
	dc:source <http://purl.org/dc/terms/> ;
	rdfs:isDefinedBy <https://spec.edmcouncil.org/cdmc/ontology/Core> ;
	rdfs:seeAlso dct:PeriodOfTime ;
	.

cdmc-core:Resource
	a owl:Class ;
	rdfs:label "Resource" ;
	rdfs:comment "resource published or curated by a single agent" ;
	dc:source <http://www.w3.org/ns/dcat#> ;
	rdfs:isDefinedBy <https://spec.edmcouncil.org/cdmc/ontology/Core> ;
	rdfs:seeAlso "" ;
	.

cdmc-core:Role
	a owl:Class ;
	rdfs:subClassOf owl:Thing ;
	rdfs:label "Role" ;
	rdfs:comment "function of a resource or agent with respect to another resource, in the context of resource attribution or resource relationships" ;
	dc:source <http://www.w3.org/ns/prov#> ;
	rdfs:isDefinedBy <https://spec.edmcouncil.org/cdmc/ontology/Core> ;
	rdfs:seeAlso <http://www.w3.org/ns/dcat#Role> ;
	.

cdmc-core:accesses
	a owl:ObjectProperty ;
	rdfs:label "accesses" ;
	rdfs:comment "identifies a Data Service accessed by an Agent." ;
	rdfs:domain cdmc-core:Agent ;
	rdfs:isDefinedBy <https://spec.edmcouncil.org/cdmc/ontology/Core> ;
	rdfs:range cdmc-core:DataService ;
	.

cdmc-core:actedOnBehalfOf
	a owl:ObjectProperty ;
	rdfs:label "acted on behalf of" ;
	rdfs:comment "identifies a subordinate Agent that acted on behalf of an accountable Agent" ;
	dc:source <http://www.w3.org/ns/prov#> ;
	rdfs:domain cdmc-core:Agent ;
	rdfs:isDefinedBy <https://spec.edmcouncil.org/cdmc/ontology/Core> ;
	rdfs:range cdmc-core:Agent ;
	.

cdmc-core:appliesTo
	a owl:ObjectProperty ;
	rdfs:label "applies to" ;
	rdfs:comment "identifies the thing to which something applies" ;
	dc:source <http://www.w3.org/ns/odrl/2/> ;
	rdfs:isDefinedBy <https://spec.edmcouncil.org/cdmc/ontology/Core> ;
	rdfs:seeAlso <http://www.w3.org/ns/odrl/2/target> ;
	.

cdmc-core:atLocation
	a owl:ObjectProperty ;
	rdfs:label "at location" ;
	rdfs:comment "specifies the Location of something" ;
	dc:source <http://www.w3.org/ns/prov#> ;
	rdfs:domain _:blank6 ;
	rdfs:isDefinedBy <https://spec.edmcouncil.org/cdmc/ontology/Core> ;
	rdfs:range cdmc-core:Location ;
	rdfs:seeAlso <http://www.w3.org/ns/prov#atLocation> ;
	.

cdmc-core:contains
	a owl:ObjectProperty ;
	rdfs:label "contains" ;
	rdfs:comment "indicates that something is included within something else" ;
	dc:source
		"CDMC" ,
		<http://www.w3.org/ns/dcat#>
		;
	rdfs:isDefinedBy <https://spec.edmcouncil.org/cdmc/ontology/Core> ;
	rdfs:seeAlso
		<http://www.w3.org/ns/odrl/2/obligation> ,
		<http://www.w3.org/ns/odrl/2/permission> ,
		<http://www.w3.org/ns/odrl/2/prohibition>
		;
	.

cdmc-core:coversLocation
	a owl:ObjectProperty ;
	rdfs:label "covers location" ;
	rdfs:comment "indicates that a Location is included in the coverage of a Resource" ;
	dc:source "CDMC" ;
	rdfs:domain cdmc-core:Resource ;
	rdfs:isDefinedBy <https://spec.edmcouncil.org/cdmc/ontology/Core> ;
	rdfs:range cdmc-core:Location ;
	.

cdmc-core:coversPeriodOfTime
	a owl:ObjectProperty ;
	rdfs:label "covers period of time" ;
	rdfs:comment "specifies the Temporal Period that a Resource covers" ;
	dc:source <http://www.w3.org/ns/dcat#> ;
	rdfs:domain cdmc-core:Resource ;
	rdfs:isDefinedBy <https://spec.edmcouncil.org/cdmc/ontology/Core> ;
	rdfs:range cdmc-core:PeriodOfTime ;
	rdfs:seeAlso dct:temporal ;
	.

cdmc-core:describes
	a owl:ObjectProperty ;
	rdfs:label "describes" ;
	rdfs:comment "indicates that something provides a description of something else" ;
	dc:source "CDMC" ;
	rdfs:isDefinedBy <https://spec.edmcouncil.org/cdmc/ontology/ControlledVocabularies> ;
	.

cdmc-core:distributedfrom
	a owl:ObjectProperty ;
	rdfs:label "distributedFrom" ;
	rdfs:comment "identifies a Distribution from which a Resource is made available" ;
	rdfs:domain cdmc-core:Distribution ;
	rdfs:isDefinedBy <https://spec.edmcouncil.org/cdmc/ontology/Core> ;
	rdfs:range cdmc-core:DatabaseStorage ;
	.

cdmc-core:excludes
	a owl:ObjectProperty ;
	rdfs:label "excludes" ;
	rdfs:comment "indicates that an instance of something is not part of a broader instance of the same thing" ;
	rdfs:domain cdmc-core:Location ;
	rdfs:isDefinedBy <https://spec.edmcouncil.org/cdmc/ontology/Core> ;
	rdfs:range cdmc-core:Location ;
	.

cdmc-core:field_aka
	a owl:AnnotationProperty ;
	rdfs:label "aka" ;
	.

cdmc-core:field_def
	a owl:AnnotationProperty ;
	rdfs:label "def" ;
	.

cdmc-core:field_group
	a owl:AnnotationProperty ;
	rdfs:label "group" ;
	.

cdmc-core:field_reference
	a owl:AnnotationProperty ;
	rdfs:label "reference" ;
	.

cdmc-core:field_src
	a owl:AnnotationProperty ;
	rdfs:label "src" ;
	.

cdmc-core:field_was
	a owl:AnnotationProperty ;
	rdfs:label "was" ;
	.

cdmc-core:hasDataService
	a owl:ObjectProperty ;
	rdfs:label "has data service" ;
	rdfs:comment "identifies a Data Service that makes a Distribution or Catalog available for consumption" ;
	dc:source <http://www.w3.org/ns/dcat#> ;
	rdfs:domain _:blank7 ;
	rdfs:isDefinedBy <https://spec.edmcouncil.org/cdmc/ontology/Core> ;
	rdfs:range cdmc-core:DataService ;
	rdfs:seeAlso <http://www.w3.org/ns/dcat#service> ;
	.

cdmc-core:hasDistribution
	a owl:ObjectProperty ;
	rdfs:label "has distribution" ;
	rdfs:comment "identifies a Distribution of a Data Set" ;
	dc:source <http://www.w3.org/ns/dcat#> ;
	rdfs:domain cdmc-core:DataSet ;
	rdfs:isDefinedBy <https://spec.edmcouncil.org/cdmc/ontology/Core> ;
	rdfs:range cdmc-core:Distribution ;
	rdfs:seeAlso <http://www.w3.org/ns/dcat#distribution> ;
	.

cdmc-core:hasExercisableAction
	a owl:ObjectProperty ;
	rdfs:label "has exercisable action" ;
	rdfs:comment "indicates that an Action is included in the coverage of a Rule or Entitlement" ;
	dc:source "CDMC" ;
	rdfs:isDefinedBy <https://spec.edmcouncil.org/cdmc/ontology/Core> ;
	rdfs:seeAlso <http://www.w3.org/ns/odrl/2/action> ;
	.

cdmc-core:hasIdentity
	a owl:ObjectProperty ;
	rdfs:label "has identity" ;
	rdfs:comment "identifies the Agent that fulfils a Role in an Agent In Role" ;
	rdfs:domain cdmc-core:AgentInRole ;
	rdfs:isDefinedBy <https://spec.edmcouncil.org/cdmc/ontology/Core> ;
	rdfs:range cdmc-core:Agent ;
	rdfs:seeAlso <https://spec.edmcouncil.org/fibo/ontology/FND/Relations/Relations/hasIdentity> ;
	.

cdmc-core:hasMediaType
	a owl:ObjectProperty ;
	rdfs:label "has media type" ;
	rdfs:comment "describes the IANA-defined media type of a Distribution" ;
	dc:source
		"CDMC" ,
		<http://www.w3.org/ns/dcat#>
		;
	rdfs:domain cdmc-core:Distribution ;
	rdfs:isDefinedBy <https://spec.edmcouncil.org/cdmc/ontology/Core> ;
	rdfs:range cdmc-core:MediaType ;
	rdfs:seeAlso <http://www.w3.org/ns/dcat#mediaType> ;
	.

cdmc-core:hasSuperset
	a owl:ObjectProperty ;
	rdfs:label "has superset" ;
	rdfs:comment "identifies a Data Set that contains at least all of the content of another Data Set" ;
	dc:source "CDMC" ;
	rdfs:domain cdmc-core:DataSet ;
	rdfs:isDefinedBy <https://spec.edmcouncil.org/cdmc/ontology/Core> ;
	rdfs:range cdmc-core:DataSet ;
	.

cdmc-core:implements
	a owl:ObjectProperty ;
	rdfs:label "implements" ;
	rdfs:comment "indicates that something is a manifestation of something more general or abstract" ;
	dc:source "CDMC" ;
	rdfs:isDefinedBy <https://spec.edmcouncil.org/cdmc/ontology/Control> ;
	.

cdmc-core:includes
	a owl:ObjectProperty ;
	rdfs:label "includes" ;
	rdfs:comment "indicates that an instance of something is part of a broader instance of the same thing" ;
	rdfs:domain cdmc-core:Location ;
	rdfs:isDefinedBy <https://spec.edmcouncil.org/cdmc/ontology/Core> ;
	rdfs:range cdmc-core:Location ;
	.

cdmc-core:isPartOf
	a owl:ObjectProperty ;
	rdfs:label "is part of" ;
	rdfs:comment "indicates that something is a constituent part of a grouping of similar things" ;
	dc:source "CDMC" ;
	rdfs:isDefinedBy <https://spec.edmcouncil.org/cdmc/ontology/Core> ;
	.

cdmc-core:isRecordFor
	a owl:ObjectProperty ;
	rdfs:label "is record for" ;
	rdfs:comment "identifies the Resource that is registered in a Catalog by a Catalog Record" ;
	dc:source
		"CDMC" ,
		<http://www.w3.org/ns/dcat#>
		;
	rdfs:domain cdmc-core:CatalogRecord ;
	rdfs:isDefinedBy <https://spec.edmcouncil.org/cdmc/ontology/Core> ;
	rdfs:range cdmc-core:Resource ;
	rdfs:seeAlso <http://xmlns.com/foaf/0.1/primaryTopic> ;
	.

cdmc-core:isResponsibleFor
	a owl:ObjectProperty ;
	rdfs:label "is responsible for" ;
	rdfs:comment "identifies a Resource that is within the scope of responsibility of an Agent In Role" ;
	rdfs:domain cdmc-core:AgentInRole ;
	rdfs:isDefinedBy <https://spec.edmcouncil.org/cdmc/ontology/Core> ;
	rdfs:range cdmc-core:Resource ;
	.

cdmc-core:playsInRole
	a owl:ObjectProperty ;
	rdfs:label "plays in role" ;
	rdfs:comment "identifies the Role that is fulfilled by an Agent in an Agent In Role" ;
	rdfs:domain cdmc-core:AgentInRole ;
	rdfs:isDefinedBy <https://spec.edmcouncil.org/cdmc/ontology/Core> ;
	rdfs:range cdmc-core:Role ;
	.

cdmc-core:references
	a owl:ObjectProperty ;
	rdfs:label "references" ;
	rdfs:comment "indicates that something makes reference to something else" ;
	dc:source "CDMC" ;
	rdfs:isDefinedBy <https://spec.edmcouncil.org/cdmc/ontology/Core> ;
	.

cdmc-core:servesDataset
	a owl:ObjectProperty ;
	rdfs:label "serves dataset" ;
	rdfs:comment "identifies a Data Set that is made available by a Data Service" ;
	dc:source <http://www.w3.org/ns/dcat#> ;
	rdfs:domain cdmc-core:DataService ;
	rdfs:isDefinedBy <https://spec.edmcouncil.org/cdmc/ontology/Core> ;
	rdfs:range cdmc-core:DataSet ;
	rdfs:seeAlso <http://www.w3.org/ns/dcat#servesDataset> ;
	.

_:blank1
	rdf:first cdmc-core:Agent ;
	rdf:rest _:blank3 ;
	.

_:blank2
	rdf:first cdmc-core:Catalog ;
	rdf:rest _:blank5 ;
	.

_:blank3
	rdf:first cdmc-core:DataService ;
	rdf:rest _:blank4 ;
	.

_:blank4
	rdf:first cdmc-core:Distribution ;
	rdf:rest rdf:nil ;
	.

_:blank5
	rdf:first cdmc-core:Distribution ;
	rdf:rest rdf:nil ;
	.

_:blank6
	a owl:Class ;
	owl:unionOf _:blank1 ;
	.

_:blank7
	a owl:Class ;
	owl:unionOf _:blank2 ;
	.

_:blank8
	a owl:Restriction ;
	owl:onProperty cdmc-core:contains ;
	owl:someValuesFrom cdmc-core:CatalogRecord ;
	.

