# imports: https://spec.edmcouncil.org/cdmc/ontology/Core

@prefix cdmc-core: <https://spec.edmcouncil.org/cdmc/ontology/Core/> .
@prefix cdmc-cost: <https://spec.edmcouncil.org/cdmc/ontology/Cost/> .
@prefix dct: <http://purl.org/dc/terms/> .
@prefix owl: <http://www.w3.org/2002/07/owl#> .
@prefix rdf: <http://www.w3.org/1999/02/22-rdf-syntax-ns#> .
@prefix rdfs: <http://www.w3.org/2000/01/rdf-schema#> .
@prefix sm: <http://www.omg.org/techprocess/ab/SpecificationMetadata/> .
@prefix xsd: <http://www.w3.org/2001/XMLSchema#> .

<https://spec.edmcouncil.org/cdmc/ontology/Cost>
	a owl:Ontology ;
	dct:abstract "This ontology defines notions for determining costs of various cloud data management functions. " ;
	dct:license "https://opensource.org/licenses/MIT"^^xsd:AnyURI ;
	sm:copyright "Copyright (c) 2022 EDM Council, Inc." ;
	owl:imports <https://spec.edmcouncil.org/cdmc/ontology/Core> ;
	owl:versionInfo "Created with TopBraid Composer" ;
	.

cdmc-cost:ComputeCost
	a owl:Class ;
	rdfs:subClassOf cdmc-cost:Cost ;
	rdfs:label "Compute Cost" ;
	rdfs:comment "cost associated with processing data" ;
	rdfs:isDefinedBy <https://spec.edmcouncil.org/cdmc/ontology/Cost> ;
	.

cdmc-cost:Cost
	a owl:Class ;
	rdfs:subClassOf cdmc-core:Metric ;
	rdfs:label "Cost" ;
	rdfs:comment "amount that has to be paid or spent to buy or obtain something" ;
	rdfs:isDefinedBy <https://spec.edmcouncil.org/cdmc/ontology/Cost> ;
	.

cdmc-cost:EgressCost
	a owl:Class ;
	rdfs:subClassOf cdmc-cost:Cost ;
	rdfs:label "Egress Cost" ;
	rdfs:comment "cost associated with data leaving a cloud defined perimeter, such as a network or storage device" ;
	rdfs:isDefinedBy <https://spec.edmcouncil.org/cdmc/ontology/Cost> ;
	.

cdmc-cost:IngressCost
	a owl:Class ;
	rdfs:subClassOf cdmc-cost:Cost ;
	rdfs:label "Ingress Cost" ;
	rdfs:comment "cost associated with data entering a cloud defined perimeter, such as a network or storage device" ;
	rdfs:isDefinedBy <https://spec.edmcouncil.org/cdmc/ontology/Cost> ;
	.

cdmc-cost:NetworkCost
	a owl:Class ;
	rdfs:subClassOf cdmc-cost:Cost ;
	rdfs:label "Network Cost" ;
	rdfs:isDefinedBy <https://spec.edmcouncil.org/cdmc/ontology/Cost> ;
	.

cdmc-cost:StorageCost
	a owl:Class ;
	rdfs:subClassOf cdmc-cost:Cost ;
	rdfs:label "Storage Cost" ;
	rdfs:comment "cost associated with storing data in a cloud defined storage device, which may be at rest or in motion" ;
	rdfs:isDefinedBy <https://spec.edmcouncil.org/cdmc/ontology/Cost> ;
	.

cdmc-cost:incurs
	a owl:ObjectProperty ;
	rdfs:label "incurs" ;
	rdfs:comment "The acquisition of a liability" ;
	rdfs:domain [] ;
	rdfs:isDefinedBy <https://spec.edmcouncil.org/cdmc/ontology/Core> ;
	rdfs:range cdmc-cost:Cost ;
	.

