# imports: https://spec.edmcouncil.org/cdmc/ontology/Core

@prefix cdmc-core: <https://spec.edmcouncil.org/cdmc/ontology/Core/> .
@prefix cdmc-du: <https://spec.edmcouncil.org/cdmc/ontology/DataUse/> .
@prefix dc: <http://purl.org/dc/elements/1.1/> .
@prefix owl: <http://www.w3.org/2002/07/owl#> .
@prefix rdf: <http://www.w3.org/1999/02/22-rdf-syntax-ns#> .
@prefix rdfs: <http://www.w3.org/2000/01/rdf-schema#> .
@prefix sm: <http://www.omg.org/techprocess/ab/SpecificationMetadata/> .
@prefix xsd: <http://www.w3.org/2001/XMLSchema#> .

<https://spec.edmcouncil.org/cdmc/ontology/DataUse>
	a owl:Ontology ;
	owl:imports <https://spec.edmcouncil.org/cdmc/ontology/Core> ;
	owl:versionInfo "Created with TopBraid Composer" ;
	.

cdmc-du:Action
	a owl:Class ;
	rdfs:subClassOf owl:Thing ;
	rdfs:label "Action" ;
	rdfs:comment "An operation that can be exercised on an Asset. An Action is associated with the Asset via the action property in a Rule." ;
	dc:source <http://www.w3.org/ns/odrl/2/> ;
	rdfs:isDefinedBy <https://spec.edmcouncil.org/cdmc/ontology/DataUse> ;
	rdfs:seeAlso "egeria:Data Processing Action" ;
	.

cdmc-du:DataSharingAgreement
	a owl:Class ;
	rdfs:subClassOf owl:Thing ;
	rdfs:label "Data Sharing Agreement" ;
	rdfs:comment "An agreement that sets out a common set of rules between the data producer and data consumer that establishes terms and restrictions of the use of consumed data." ;
	dc:source "DCAM" ;
	rdfs:isDefinedBy <https://spec.edmcouncil.org/cdmc/ontology/DataUse> ;
	.

cdmc-du:Entitlement
	a owl:Class ;
	rdfs:subClassOf
		owl:Thing ,
		_:blank1 ,
		_:blank2
		;
	rdfs:label "Entitlement" ;
	rdfs:comment "A status granted to a person or group of persons representing their permission to access a specific data asset or any data asset with specific scope and characteristics." ;
	rdfs:isDefinedBy <https://spec.edmcouncil.org/cdmc/ontology/DataUse> ;
	.

cdmc-du:Purpose
	a owl:Class ;
	rdfs:subClassOf owl:Thing ;
	rdfs:label "Purpose" ;
	rdfs:comment "A reason for which an action is performed." ;
	rdfs:isDefinedBy <https://spec.edmcouncil.org/cdmc/ontology/DataUse> ;
	rdfs:seeAlso "egeria:Data Processing Purpose" ;
	.

cdmc-du:ServiceLevelAgreement
	a owl:Class ;
	rdfs:subClassOf
		owl:Thing ,
		_:blank3
		;
	rdfs:label "Service Level Agreement" ;
	rdfs:comment "An overall agreement with a provider on what is provided, how it is supported, times, locations, costs, performance, responsibilities, etc." ;
	dc:source "CDMC Training Materials" ;
	rdfs:isDefinedBy <https://spec.edmcouncil.org/cdmc/ontology/DataUse> ;
	.

cdmc-du:ServiceLevelObjective
	a owl:Class ;
	rdfs:subClassOf owl:Thing ;
	rdfs:label "Service Level Objective" ;
	rdfs:comment "A component of the SLA covering measurable (quantifiable) aspects of the agreement to objectively monitor performance of the provider against the overall agreement." ;
	dc:source "CDMC Training Materials" ;
	rdfs:isDefinedBy <https://spec.edmcouncil.org/cdmc/ontology/DataUse> ;
	.

cdmc-du:Usage
	a owl:Class ;
	rdfs:subClassOf
		owl:Thing ,
		_:blank4
		;
	rdfs:label "Usage" ;
	rdfs:comment "Use of a Data Asset by an Agent via a Data Service for one or more specified Purposes" ;
	rdfs:isDefinedBy <https://spec.edmcouncil.org/cdmc/ontology/DataUse> ;
	rdfs:seeAlso "egeria:Data Processing Description" ;
	.

cdmc-du:applicableIn
	a owl:ObjectProperty ;
	rdfs:label "applicable in" ;
	rdfs:domain cdmc-du:Entitlement ;
	rdfs:isDefinedBy <https://spec.edmcouncil.org/cdmc/ontology/DataUse> ;
	rdfs:range cdmc-core:Location ;
	.

cdmc-du:authorizes
	a owl:ObjectProperty ;
	rdfs:label "authorizes" ;
	rdfs:domain cdmc-du:Entitlement ;
	rdfs:isDefinedBy <https://spec.edmcouncil.org/cdmc/ontology/DataUse> ;
	rdfs:range cdmc-core:Agent ;
	.

cdmc-du:constrains
	a owl:ObjectProperty ;
	rdfs:label "constrains" ;
	rdfs:comment """The fact
 that a concept acts as a constraint upon another concept""" ;
	rdfs:domain cdmc-du:DataSharingAgreement ;
	rdfs:isDefinedBy <https://spec.edmcouncil.org/cdmc/ontology/DataUse> ;
	rdfs:range cdmc-du:Purpose ;
	.

cdmc-du:exercisedAction
	a owl:ObjectProperty ;
	rdfs:label "exercised action" ;
	rdfs:comment "The exercising of an Action by a Usage" ;
	rdfs:domain cdmc-du:Usage ;
	rdfs:isDefinedBy <https://spec.edmcouncil.org/cdmc/ontology/DataUse> ;
	rdfs:range cdmc-du:Action ;
	.

cdmc-du:hasServiceLevelAgreement
	a owl:ObjectProperty ;
	rdfs:label "has service level agreement" ;
	rdfs:comment "Indicates one or more SLA instances are includes as part of a Data Sharing Agreement." ;
	dc:source "CDMC" ;
	rdfs:domain cdmc-du:DataSharingAgreement ;
	rdfs:isDefinedBy <https://spec.edmcouncil.org/cdmc/ontology/DataUse> ;
	rdfs:range cdmc-du:ServiceLevelAgreement ;
	.

cdmc-du:informed
	a owl:ObjectProperty ;
	rdfs:label "informed" ;
	rdfs:domain cdmc-core:DataService ;
	rdfs:isDefinedBy <https://spec.edmcouncil.org/cdmc/ontology/Core> ;
	rdfs:range cdmc-du:Usage ;
	.

cdmc-du:usedBy
	a owl:ObjectProperty ;
	rdfs:label "used by" ;
	rdfs:comment "The indication of the Agent associated with a Usage" ;
	rdfs:domain cdmc-du:Usage ;
	rdfs:isDefinedBy <https://spec.edmcouncil.org/cdmc/ontology/DataUse> ;
	rdfs:range cdmc-core:Agent ;
	.

cdmc-du:usedFor
	a owl:ObjectProperty ;
	rdfs:label "used for" ;
	rdfs:comment "The association of a Purpose with a Usage" ;
	rdfs:domain cdmc-du:Usage ;
	rdfs:isDefinedBy <https://spec.edmcouncil.org/cdmc/ontology/DataUse> ;
	rdfs:range cdmc-du:Purpose ;
	.

_:blank1
	a owl:Restriction ;
	owl:onProperty cdmc-core:hasExercisableAction ;
	owl:allValuesFrom cdmc-du:Action ;
	.

_:blank2
	a owl:Restriction ;
	owl:onProperty cdmc-core:appliesTo ;
	owl:someValuesFrom cdmc-core:DataService ;
	.

_:blank3
	a owl:Restriction ;
	owl:onProperty cdmc-core:contains ;
	owl:someValuesFrom cdmc-du:ServiceLevelObjective ;
	.

_:blank4
	a owl:Restriction ;
	owl:onProperty cdmc-core:describes ;
	owl:someValuesFrom cdmc-core:DataService ;
	.

