# imports: https://spec.edmcouncil.org/cdmc/ontology/ControlledVocabularies
# imports: https://spec.edmcouncil.org/cdmc/ontology/Core

@prefix cdmc-core: <https://spec.edmcouncil.org/cdmc/ontology/Core/> .
@prefix cdmc-cv: <https://spec.edmcouncil.org/cdmc/ontology/ControlledVocabularies/> .
@prefix cdmc-dq: <https://spec.edmcouncil.org/cdmc/ontology/DataQuality/> .
@prefix dc: <http://purl.org/dc/elements/1.1/> .
@prefix dct: <http://purl.org/dc/terms/> .
@prefix owl: <http://www.w3.org/2002/07/owl#> .
@prefix rdf: <http://www.w3.org/1999/02/22-rdf-syntax-ns#> .
@prefix rdfs: <http://www.w3.org/2000/01/rdf-schema#> .
@prefix sm: <http://www.omg.org/techprocess/ab/SpecificationMetadata/> .
@prefix xsd: <http://www.w3.org/2001/XMLSchema#> .

<https://spec.edmcouncil.org/cdmc/ontology/DataQuality>
	a owl:Ontology ;
	dct:abstract "This ontology provides concepts for measuring and controlling data quality.  " ;
	dct:license "https://opensource.org/licenses/MIT"^^xsd:AnyURI ;
	sm:copyright "Copyright (c) 2022 EDM Council, Inc." ;
	owl:imports
		<https://spec.edmcouncil.org/cdmc/ontology/ControlledVocabularies> ,
		<https://spec.edmcouncil.org/cdmc/ontology/Core>
		;
	owl:versionInfo "Created with TopBraid Composer" ;
	.

cdmc-dq:BusinessContext
	a owl:Class ;
	rdfs:subClassOf owl:Thing ;
	rdfs:label "Business Context" ;
	dc:source "CDMC" ;
	rdfs:isDefinedBy <https://spec.edmcouncil.org/cdmc/ontology/DataQuality> ;
	<http://www.w3.org/2004/02/skos/core#definition> "scoping for rules or concepts related to a particular business domain (could represent a company, an organization, or a particular project, for example)" ;
	.

cdmc-dq:DataQualityAssessment
	a owl:Class ;
	rdfs:subClassOf owl:Thing ;
	rdfs:label "Data Quality Assessment" ;
	dc:source "CDMC" ;
	rdfs:isDefinedBy <https://spec.edmcouncil.org/cdmc/ontology/DataQuality> ;
	<http://www.w3.org/2004/02/skos/core#definition> "results of an evaluation of a given Data Quality Execution Rule against a particular Data Quality Measurement, determining whether a measurement successfully meets the constraints of the rule" ;
	.

cdmc-dq:DataQualityDimension
	a owl:Class ;
	rdfs:subClassOf owl:Thing ;
	rdfs:label "Data Quality Dimension" ;
	dc:source "DCAM Glossary" ;
	rdfs:isDefinedBy <https://spec.edmcouncil.org/cdmc/ontology/DataQuality> ;
	rdfs:seeAlso <http://www.w3.org/ns/dqv#Dimension> ;
	<http://www.w3.org/2004/02/skos/core#definition> "category of measurement used to evaluate the degree to which data is fit-for-purpose" ;
	.

cdmc-dq:DataQualityDimensionCategory
	a owl:Class ;
	rdfs:subClassOf owl:Thing ;
	rdfs:label "Data Quality Dimension Category" ;
	dc:source <http://www.w3.org/ns/dqv#> ;
	rdfs:isDefinedBy <https://spec.edmcouncil.org/cdmc/ontology/DataQuality> ;
	<http://www.w3.org/2004/02/skos/core#definition> "group of quality dimensions in which a common type of information is used as quality indicator" ;
	.

cdmc-dq:DataQualityExecutionRule
	a owl:Class ;
	rdfs:subClassOf
		owl:Thing ,
		_:blank3
		;
	rdfs:label "Data Quality Execution Rule" ;
	dc:source
		"CDMC" ,
		"DCAM Glossary"
		;
	rdfs:isDefinedBy <https://spec.edmcouncil.org/cdmc/ontology/DataQuality> ;
	<http://www.w3.org/2004/02/skos/core#definition> "specific algorithm or logic that can be executed to implement a Data Quality Rule" ;
	.

cdmc-dq:DataQualityMeasurement
	a owl:Class ;
	rdfs:subClassOf owl:Thing ;
	rdfs:label "Data Quality Measurement" ;
	dc:source <http://www.w3.org/ns/dqv#> ;
	rdfs:isDefinedBy <https://spec.edmcouncil.org/cdmc/ontology/DataQuality> ;
	rdfs:seeAlso <http://www.w3.org/ns/dqv#QualityMeasurement> ;
	<http://www.w3.org/2004/02/skos/core#definition> "evaluation of a given data asset against a specific quality metric" ;
	.

cdmc-dq:DataQualityMetric
	a owl:Class ;
	rdfs:subClassOf cdmc-core:Metric ;
	rdfs:label "Data Quality Metric" ;
	dc:source <http://www.w3.org/ns/dqv#> ;
	rdfs:isDefinedBy <https://spec.edmcouncil.org/cdmc/ontology/DataQuality> ;
	rdfs:seeAlso <http://www.w3.org/ns/dqv#Metric> ;
	<http://www.w3.org/2004/02/skos/core#definition> "standard to measure a quality dimension. An observation (instance of Data Quality Measurement) assigns a value in a given unit to a Metric" ;
	.

cdmc-dq:DataQualityReport
	a owl:Class ;
	rdfs:subClassOf
		owl:Thing ,
		_:blank2
		;
	rdfs:label "Data Quality Report" ;
	rdfs:isDefinedBy <https://spec.edmcouncil.org/cdmc/ontology/DataQuality> ;
	<http://www.w3.org/2004/02/skos/core#definition> "report that combines Data Quality Assessments to convey the overall data quality of a Data Asset" ;
	.

cdmc-dq:DataQualityRule
	a owl:Class ;
	rdfs:subClassOf
		owl:Thing ,
		_:blank1 ,
		_:blank4
		;
	rdfs:label "Data Quality Rule" ;
	dc:source "DCAM Glossary" ;
	rdfs:isDefinedBy <https://spec.edmcouncil.org/cdmc/ontology/DataQuality> ;
	<http://www.w3.org/2004/02/skos/core#definition> "statement that applies an algorithm or logic to a data value to measure the fit-for-purpose of the value" ;
	.

cdmc-dq:inBusinessContext
	a owl:ObjectProperty ;
	rdfs:label "in business context" ;
	dc:source "CDMC" ;
	rdfs:domain cdmc-dq:DataQualityRule ;
	rdfs:isDefinedBy <https://spec.edmcouncil.org/cdmc/ontology/DataQuality> ;
	rdfs:range cdmc-dq:BusinessContext ;
	<http://www.w3.org/2004/02/skos/core#definition> "indicates a Business Context in which a Data Quality Rule is to be applied" ;
	.

cdmc-dq:inDataQualityDimension
	a owl:ObjectProperty ;
	rdfs:label "in data quality dimension" ;
	dc:source <http://www.w3.org/ns/dqv#> ;
	rdfs:domain cdmc-dq:DataQualityMetric ;
	rdfs:isDefinedBy <https://spec.edmcouncil.org/cdmc/ontology/DataQuality> ;
	rdfs:range cdmc-dq:DataQualityDimension ;
	rdfs:seeAlso <http://www.w3.org/ns/dqv#inDimension> ;
	<http://www.w3.org/2004/02/skos/core#definition> "represents the Data Quality Dimension that a Data Quality Metric allows measurement of" ;
	.

cdmc-dq:inDataQualityDimensionCategory
	a owl:ObjectProperty ;
	rdfs:label "in data quality dimension category" ;
	dc:source <http://www.w3.org/ns/dqv#> ;
	rdfs:domain cdmc-dq:DataQualityDimension ;
	rdfs:isDefinedBy <https://spec.edmcouncil.org/cdmc/ontology/DataQuality> ;
	rdfs:range cdmc-dq:DataQualityDimensionCategory ;
	<http://www.w3.org/2004/02/skos/core#definition> "associates a Data Quality Dimension Category with a Data Quality Dimension" ;
	.

cdmc-dq:isAssessmentOfMeasurement
	a owl:ObjectProperty ;
	rdfs:label "is assessment of measurement" ;
	dc:source "CDMC" ;
	rdfs:domain cdmc-dq:DataQualityAssessment ;
	rdfs:isDefinedBy <https://spec.edmcouncil.org/cdmc/ontology/DataQuality> ;
	rdfs:range cdmc-dq:DataQualityMeasurement ;
	<http://www.w3.org/2004/02/skos/core#definition> "identifies a Data Quality Measurement included within a Data Quality Assessment" ;
	.

cdmc-dq:isMeasurementOfDataQualityMetric
	a owl:ObjectProperty ;
	rdfs:label "is measurement of data quality metric" ;
	dc:source <http://www.w3.org/ns/dqv#> ;
	rdfs:domain cdmc-dq:DataQualityMeasurement ;
	rdfs:isDefinedBy <https://spec.edmcouncil.org/cdmc/ontology/DataQuality> ;
	rdfs:range cdmc-dq:DataQualityMetric ;
	rdfs:seeAlso <http://www.w3.org/ns/dqv#isMeasurementOf> ;
	<http://www.w3.org/2004/02/skos/core#definition> "indicates the Data Quality Metric being observed by a Data Quality Measurement" ;
	.

cdmc-dq:isMeasurementOfResource
	a owl:ObjectProperty ;
	rdfs:label "is measurement of resource" ;
	dc:source <http://www.w3.org/ns/dqv#> ;
	rdfs:domain cdmc-dq:DataQualityMeasurement ;
	rdfs:isDefinedBy <https://spec.edmcouncil.org/cdmc/ontology/DataQuality> ;
	rdfs:range cdmc-core:Resource ;
	<http://www.w3.org/2004/02/skos/core#definition> "identifies the Resource on which a Data Quality Measurement is performed" ;
	.

cdmc-dq:isRequirementForMetric
	a owl:ObjectProperty ;
	rdfs:label "is requirement for metric" ;
	dc:source "CDMC" ;
	rdfs:domain cdmc-dq:DataQualityExecutionRule ;
	rdfs:isDefinedBy <https://spec.edmcouncil.org/cdmc/ontology/DataQuality> ;
	rdfs:range cdmc-dq:DataQualityMetric ;
	<http://www.w3.org/2004/02/skos/core#definition> "identifies a Data Quality Metric that a Data Quality Execution Rule is involved in the production of" ;
	.

cdmc-dq:reportsDataQualityFor
	a owl:ObjectProperty ;
	rdfs:label "reports data quality for" ;
	rdfs:domain cdmc-dq:DataQualityReport ;
	rdfs:isDefinedBy <https://spec.edmcouncil.org/cdmc/ontology/DataQuality> ;
	rdfs:range cdmc-core:Resource ;
	<http://www.w3.org/2004/02/skos/core#definition> "identifies a Resource that is the subject of a Data Quality Report" ;
	.

cdmc-dq:wasAssessedAgainstRequirement
	a owl:ObjectProperty ;
	rdfs:label "was assessed against requirement" ;
	dc:source "CDMC" ;
	rdfs:domain cdmc-dq:DataQualityAssessment ;
	rdfs:isDefinedBy <https://spec.edmcouncil.org/cdmc/ontology/DataQuality> ;
	rdfs:range cdmc-dq:DataQualityExecutionRule ;
	<http://www.w3.org/2004/02/skos/core#definition> "identifies the Data Quality Execution Rule against which a Data Quality Assessment was performed" ;
	.

_:blank1
	a owl:Restriction ;
	owl:onProperty cdmc-core:appliesTo ;
	owl:someValuesFrom cdmc-cv:DataElementConcept ;
	.

_:blank2
	a owl:Restriction ;
	owl:onProperty cdmc-core:contains ;
	owl:someValuesFrom cdmc-dq:DataQualityAssessment ;
	.

_:blank3
	a owl:Restriction ;
	owl:onProperty cdmc-core:implements ;
	owl:someValuesFrom cdmc-dq:DataQualityRule ;
	.

_:blank4
	a owl:Restriction ;
	owl:onProperty cdmc-core:references ;
	owl:someValuesFrom cdmc-dq:DataQualityDimension ;
	.

