# imports: https://spec.edmcouncil.org/cdmc/ontology/Core

@prefix cdmc-core: <https://spec.edmcouncil.org/cdmc/ontology/Core/> .
@prefix cdmc-lin: <https://spec.edmcouncil.org/cdmc/ontology/Lineage/> .
@prefix dc: <http://purl.org/dc/elements/1.1/> .
@prefix dct: <http://purl.org/dc/terms/> .
@prefix owl: <http://www.w3.org/2002/07/owl#> .
@prefix rdf: <http://www.w3.org/1999/02/22-rdf-syntax-ns#> .
@prefix rdfs: <http://www.w3.org/2000/01/rdf-schema#> .
@prefix skos: <http://www.w3.org/2004/02/skos/core#> .
@prefix sm: <http://www.omg.org/techprocess/ab/SpecificationMetadata/> .
@prefix xsd: <http://www.w3.org/2001/XMLSchema#> .

<https://spec.edmcouncil.org/cdmc/ontology/Lineage>
	a owl:Ontology ;
	dct:abstract "This ontology provides concepts and relationships for tracking lineage of data in cloud data management. " ;
	dct:license "https://opensource.org/licenses/MIT"^^xsd:AnyURI ;
	sm:copyright "Copyright (c) 2022 EDM Council, Inc." ;
	owl:imports <https://spec.edmcouncil.org/cdmc/ontology/Core> ;
	owl:versionInfo "Created with TopBraid Composer" ;
	.

cdmc-lin:Activity
	a owl:Class ;
	rdfs:subClassOf owl:Thing ;
	rdfs:label "Activity" ;
	dc:source <http://www.w3.org/ns/prov#> ;
	rdfs:isDefinedBy <https://spec.edmcouncil.org/cdmc/ontology/Lineage> ;
	rdfs:seeAlso <http://www.w3.org/ns/prov#Activity> ;
	skos:definition "something that occurs over a period of time and acts upon or with entities" ;
	skos:example "may include consuming, processing, transforming, modifying, relocating, using, or generating entities" ;
	.

cdmc-lin:Derivation
	a owl:Class ;
	rdfs:subClassOf owl:Thing ;
	rdfs:label "Derivation" ;
	dc:source <http://www.w3.org/ns/prov#> ;
	rdfs:isDefinedBy <https://spec.edmcouncil.org/cdmc/ontology/Lineage> ;
	rdfs:seeAlso <http://www.w3.org/ns/prov#Derivation> ;
	skos:definition "derivation is a transformation of an entity into another, an update of an entity resulting in a new one, or the creation of a new entity as a copy of a pre-existing entity" ;
	.

cdmc-lin:Entity
	a owl:Class ;
	rdfs:subClassOf owl:Thing ;
	rdfs:label "Entity" ;
	dc:source <http://www.w3.org/ns/prov#> ;
	rdfs:isDefinedBy <https://spec.edmcouncil.org/cdmc/ontology/Lineage> ;
	rdfs:seeAlso <http://www.w3.org/ns/prov#Entity> ;
	owl:equivalentClass _:blank3 ;
	skos:definition "entity is a physical, digital, conceptual, or other kind of thing with some fixed aspects; entities may be real or imaginary" ;
	.

cdmc-lin:LineageRecord
	a owl:Class ;
	rdfs:subClassOf
		owl:Thing ,
		_:blank4
		;
	rdfs:label "Lineage Record" ;
	rdfs:isDefinedBy <https://spec.edmcouncil.org/cdmc/ontology/Lineage> ;
	skos:definition "information about the movement and transformation of data from a point of origin to its final destination" ;
	.

cdmc-lin:LineageReport
	a owl:Class ;
	rdfs:subClassOf owl:Thing ;
	rdfs:label "Lineage Report" ;
	rdfs:isDefinedBy <https://spec.edmcouncil.org/cdmc/ontology/Lineage> ;
	skos:definition "report that provides information about a number of movements and transformations of data from a point of origin to its final destination" ;
	.

cdmc-lin:Revision
	a owl:Class ;
	rdfs:subClassOf cdmc-lin:Derivation ;
	rdfs:label "Revision" ;
	dc:source <http://www.w3.org/ns/prov#> ;
	rdfs:isDefinedBy <https://spec.edmcouncil.org/cdmc/ontology/Lineage> ;
	rdfs:seeAlso <http://www.w3.org/ns/prov#Revision> ;
	skos:definition "revision is a derivation for which the resulting entity is a revised version of some original" ;
	.

cdmc-lin:derivedFromEntity
	a owl:ObjectProperty ;
	rdfs:label "derived from entity" ;
	dc:source
		"CDMC" ,
		"prov:"
		;
	rdfs:domain cdmc-lin:Derivation ;
	rdfs:isDefinedBy <https://spec.edmcouncil.org/cdmc/ontology/Lineage> ;
	rdfs:range cdmc-lin:Entity ;
	rdfs:seeAlso <http://www.w3.org/ns/prov#entity> ;
	skos:definition "identifies an Entity that is an input to a Derivation" ;
	.

cdmc-lin:hadActivity
	a owl:ObjectProperty ;
	rdfs:label "had activity" ;
	dc:source <http://www.w3.org/ns/prov#> ;
	rdfs:domain cdmc-lin:Derivation ;
	rdfs:isDefinedBy <https://spec.edmcouncil.org/cdmc/ontology/Lineage> ;
	rdfs:range cdmc-lin:Activity ;
	rdfs:seeAlso <http://www.w3.org/ns/prov#hadActivity> ;
	skos:definition "identifes an Activity that is involved in a Derivation" ;
	.

cdmc-lin:hadDuration
	a owl:ObjectProperty ;
	rdfs:label "had duration" ;
	dc:source "CDMC" ;
	rdfs:domain cdmc-lin:Activity ;
	rdfs:isDefinedBy <https://spec.edmcouncil.org/cdmc/ontology/Lineage> ;
	rdfs:range cdmc-core:PeriodOfTime ;
	skos:definition "specifies the Period of Time over which an Activity took place" ;
	.

cdmc-lin:hasCreator
	a owl:ObjectProperty ;
	rdfs:label "has creator" ;
	dc:source
		"CDMC" ,
		<http://purl.org/dc/terms/>
		;
	rdfs:domain cdmc-lin:Entity ;
	rdfs:isDefinedBy <https://spec.edmcouncil.org/cdmc/ontology/Lineage> ;
	rdfs:range cdmc-core:Agent ;
	rdfs:seeAlso dct:creator ;
	skos:definition "identifies the Agent responsible for the creation of an Entity" ;
	.

cdmc-lin:hasPublisher
	a owl:ObjectProperty ;
	rdfs:label "has publisher" ;
	dc:source
		"CDMC" ,
		<http://purl.org/dc/terms/>
		;
	rdfs:domain cdmc-lin:Entity ;
	rdfs:isDefinedBy <https://spec.edmcouncil.org/cdmc/ontology/Lineage> ;
	rdfs:range cdmc-core:Agent ;
	rdfs:seeAlso dct:publisher ;
	skos:definition "identifies the Agent responsible for making an Entity available for consumption" ;
	.

cdmc-lin:hasQualifiedDerivation
	a owl:ObjectProperty ;
	rdfs:label "has qualified derivation" ;
	dc:source <http://www.w3.org/ns/prov#> ;
	rdfs:domain cdmc-lin:Entity ;
	rdfs:isDefinedBy <https://spec.edmcouncil.org/cdmc/ontology/Lineage> ;
	rdfs:range cdmc-lin:Derivation ;
	rdfs:seeAlso <http://www.w3.org/ns/prov#qualifiedDerivation> ;
	skos:definition "identifies a Derivation that has influenced the creation or modification of an Entity" ;
	.

cdmc-lin:isRevisionOf
	a owl:ObjectProperty ;
	rdfs:label "is revision of" ;
	dc:source <http://www.w3.org/ns/prov#> ;
	rdfs:domain cdmc-lin:Entity ;
	rdfs:isDefinedBy <https://spec.edmcouncil.org/cdmc/ontology/Lineage> ;
	rdfs:range cdmc-lin:Entity ;
	rdfs:seeAlso <http://www.w3.org/ns/prov#wasRevisionOf> ;
	skos:definition "indicates that an Entity is a revised version of another Entity" ;
	.

cdmc-lin:isSpecializationOf
	a owl:ObjectProperty ;
	rdfs:label "is specialization of" ;
	dc:source <http://www.w3.org/ns/prov#> ;
	rdfs:domain cdmc-lin:Entity ;
	rdfs:isDefinedBy <https://spec.edmcouncil.org/cdmc/ontology/Lineage> ;
	rdfs:range cdmc-lin:Entity ;
	rdfs:seeAlso <http://www.w3.org/ns/prov#specializationOf> ;
	skos:definition "indicates that an entity that is a specialization of another Entity, sharing all aspects of the latter and additionally presenting more specific aspects of it" ;
	.

cdmc-lin:recordedBy
	a owl:ObjectProperty ;
	rdfs:label "recorded by" ;
	rdfs:domain cdmc-lin:LineageRecord ;
	rdfs:isDefinedBy <https://spec.edmcouncil.org/cdmc/ontology/Lineage> ;
	rdfs:range cdmc-core:Agent ;
	skos:definition "identifies the Agent that produced a Lineage Record" ;
	.

cdmc-lin:records
	a owl:ObjectProperty ;
	rdfs:label "records" ;
	rdfs:domain cdmc-lin:LineageRecord ;
	rdfs:isDefinedBy <https://spec.edmcouncil.org/cdmc/ontology/Lineage> ;
	rdfs:range cdmc-lin:Derivation ;
	skos:definition "identifies a Derivation that is documented by a Lineage Record" ;
	.

cdmc-lin:wasAssociatedWith
	a owl:ObjectProperty ;
	rdfs:label "was associated with" ;
	dc:source <http://www.w3.org/ns/prov#> ;
	rdfs:domain cdmc-lin:Activity ;
	rdfs:isDefinedBy <https://spec.edmcouncil.org/cdmc/ontology/Lineage> ;
	rdfs:range cdmc-core:Agent ;
	rdfs:seeAlso <http://www.w3.org/ns/prov#wasAssociatedWith> ;
	skos:definition "indicates that an Agent played a role in an Activity" ;
	.

cdmc-lin:wasAttributedTo
	a owl:ObjectProperty ;
	rdfs:label "was attributed to" ;
	dc:source <http://www.w3.org/ns/prov#> ;
	rdfs:domain cdmc-lin:Entity ;
	rdfs:isDefinedBy <https://spec.edmcouncil.org/cdmc/ontology/Lineage> ;
	rdfs:range cdmc-core:Agent ;
	rdfs:seeAlso <http://www.w3.org/ns/prov#wasAttributedTo> ;
	skos:definition "indicates that an Agent played a role the creation, change or deletion of an Entity" ;
	.

cdmc-lin:wasDerivedFrom
	a owl:ObjectProperty ;
	rdfs:label "was derived from" ;
	dc:source <http://www.w3.org/ns/prov#> ;
	rdfs:domain cdmc-lin:Entity ;
	rdfs:isDefinedBy <https://spec.edmcouncil.org/cdmc/ontology/Lineage> ;
	rdfs:range cdmc-lin:Entity ;
	rdfs:seeAlso <http://www.w3.org/ns/prov#wasDerivedFrom> ;
	skos:definition "indicates than an Entity is the result of the transformation or update of another Entity" ;
	.

cdmc-lin:wasGeneratedBy
	a owl:ObjectProperty ;
	rdfs:label "was generated by" ;
	dc:source <http://www.w3.org/ns/prov#> ;
	rdfs:domain cdmc-lin:Entity ;
	rdfs:isDefinedBy <https://spec.edmcouncil.org/cdmc/ontology/Lineage> ;
	rdfs:range cdmc-lin:Activity ;
	rdfs:seeAlso <http://www.w3.org/ns/prov#wasGeneratedBy> ;
	skos:definition "indicates than an Entity has been created as the result of an Activity" ;
	.

cdmc-lin:wasInformedBy
	a owl:ObjectProperty ;
	rdfs:label "was informed by" ;
	dc:source <http://www.w3.org/ns/prov#> ;
	rdfs:domain cdmc-lin:Activity ;
	rdfs:isDefinedBy <https://spec.edmcouncil.org/cdmc/ontology/Lineage> ;
	rdfs:range cdmc-lin:Activity ;
	rdfs:seeAlso <http://www.w3.org/ns/prov#wasInformedBy> ;
	skos:definition "indicates that an Activity involved the exchange of an Entity with another Activity" ;
	.

_:blank1
	rdf:first cdmc-core:Agent ;
	rdf:rest _:blank2 ;
	.

_:blank2
	rdf:first cdmc-core:Resource ;
	rdf:rest rdf:nil ;
	.

_:blank3
	a owl:Class ;
	owl:unionOf _:blank1 ;
	.

_:blank4
	a owl:Restriction ;
	owl:onProperty cdmc-core:isPartOf ;
	owl:someValuesFrom cdmc-lin:LineageReport ;
	.

